Test/dafny0/OpaqueFunctions.dfy
@@ -1,0 +1,123 @@
+module A {
+  class C {
+    var x: int;
+    predicate Valid()
+      reads this;
+    {
+      0 <= x
+    }
+    function Get(): int
+      reads this;
+    {
+      x
+    }
+    constructor ()
+      modifies this;
+      ensures Valid();
+    {
+      x := 8;
+    }
+    method M()
+      requires Valid();
+    {
+      assert Get() == x;
+      assert x == 8;  // error
+    }
+  }
+}
+module A' refines A {
+  class C {
+    predicate Valid...
+    {
+      x == 8
+    }
+    method N()
+      requires Valid();
+    {
+      assert Get() == x;
+      assert x == 8;
+    }
+  }
+}
+
+module B {
+  import X as A
+  method Main() {
+    var c := new X.C();
+    c.M();  // fine
+    c.x := c.x + 1;
+    c.M();  // error, because Valid() is opaque
+  }
+  method L(c: X.C)
+    requires c != null;
+    modifies c;
+  {
+    assert c.Get() == c.x;  // error because Get() s opaque
+    if * {
+      assert c.Valid();  // error, because Valid() is opaque
+    } else if * {
+      c.x := 7;
+      assert c.Valid();  // error, because Valid() is opaque
+    } else {
+      c.x := 8;
+      assert c.Valid();  // error, because Valid() is opaque
+    }
+  }
+}
+module B_direct {
+  import X as A'
+  method Main() {
+    var c := new X.C();
+    c.M();  // fine
+    c.x := c.x + 1;
+    if * {
+      assert c.Valid();  // error, because Valid() is opaque
+    } else {
+      c.M();  // error, because Valid() is opaque
+    }
+  }
+  method L(c: X.C)
+    requires c != null;
+    modifies c;
+  {
+    assert c.Get() == c.x;  // error because Get() s opaque
+    if * {
+      assert c.Valid();  // error, because Valid() is opaque
+    } else if * {
+      c.x := 7;
+      assert c.Valid();  // error, because Valid() is opaque
+    } else {
+      c.x := 8;
+      assert c.Valid();  // error, because Valid() is opaque
+    }
+  }
+}
+module B' refines B {
+  import X = A'  // this by itself produces no more error
+  method Main'() {
+    var c := new X.C();
+    c.M();  // fine
+    c.x := c.x + 1;
+    if * {
+      assert c.Valid();  // error, because Valid() is opaque
+    } else {
+      c.M();  // error, because Valid() is opaque
+    }
+  }
+  method L'(c: X.C)
+    requires c != null;
+    modifies c;
+  {
+    assert c.Get() == c.x;  // error because Get() s opaque
+    if * {
+      assert c.Valid();  // error, because Valid() is opaque
+    } else if * {
+      c.x := 7;
+      assert c.Valid();  // error, because Valid() is opaque
+    } else {
+      c.x := 8;
+      assert c.Valid();  // error, because Valid() is opaque
+    }
+  }
+}
+
